
$$
\begin{align}
y &= C_1e^{\alpha x + i\beta x} + C_2 e^{\alpha x - i\beta x} \\
\\
&= e^{\alpha x}(C_1 e^{i\beta x} + C_2 e^{-i\beta x}) \\\\
&= e^{\alpha x}\Big(C_1(\cos{\beta x} + i\sin{\beta x}) + C_2(\cos{\beta x} - i\sin{\beta x})\Big) \\\\
&= e^{\alpha x}(c_1\cos{\beta x} + c_2\sin{\beta x}) \qquad \qquad(c_1 = C_1 + C_2, \quad c_2 = C_1 - C_2)
\end{align}
$$
---
note :

$$
\begin{gather}
e^{ix} = \cos x + i\sin x\\\\\
\sin(x) = \frac{e^{ix} - e^{-ix}}{2i} \\\\
\cos(x) = \frac{e^{ix} + e^{-ix}}{2} \\
\end{gather}
$$